\documentclass[12pt]{article}
\usepackage{fullpage,enumitem,amsmath,amssymb,graphicx}

\begin{document}

\begin{center}
{\Large CSED342 Assignment 8 \vspace{10pt}}

\begin{tabular}{rl}
Student ID: & 20210212 \\
Name: & Jimin Lee \\
\end{tabular}
\end{center}

\begin{center}
By turning in this assignment, I agree by the POSTECH honor code and declare that all of this is my own work.
\end{center}

\section*{Problem 2a}
$KB = \{(A \land B) \xrightarrow{} \neg C, \neg(\neg A \lor C) \xrightarrow{} D, A\}$ \\
\begin{enumerate}[label=(\roman*)]
    \item\text First, let's convert this $KB$ into CNF forms.
        \begin{align*}
            {(A \land B) \xrightarrow{} \neg C} \quad &\Rightarrow \quad {\neg(A \lor B) \lor \neg C} \quad \\&\Rightarrow \quad {(\neg A \land \neg B) \lor \neg C} \quad \\&\Rightarrow \quad {(\neg A \lor \neg C) \land (\neg B \lor \neg C)} \quad \\&\Rightarrow \quad {\neg A \lor \neg C, \quad \neg B \lor \neg C} \\ \\
            {\neg(\neg A \lor C) \xrightarrow{} D} \quad &\Rightarrow \quad {\neg A \lor C \lor D}
        \end{align*}
    $KB = \{{\neg A \lor \neg C, \neg B \lor \neg C}, {\neg A \lor C \lor D}, A\}$ \\
    \item\text Secondly, let's apply Modus Ponens inference rule. \\
        \begin{align*}
            \frac{A, \neg A \lor \neg C}{\neg C} \quad &\Rightarrow \quad KB = \{{\neg A \lor \neg C, \neg B \lor \neg C}, {\neg A \lor C \lor D}, A,\neg C\} \\
            \frac{A, \neg A \lor C \lor D}{C \lor D} \quad &\Rightarrow \quad KB = \{{\neg A \lor \neg C, \neg B \lor \neg C}, {\neg A \lor C \lor D}, A,\neg C, C \lor D\} \\
            \frac{\neg C, C \lor D}{D} \quad &\Rightarrow \quad KB = \{{\neg A \lor \neg C, \neg B \lor \neg C}, {\neg A \lor C \lor D}, A,\neg C, C \lor D, D\} \\
        \end{align*}
\end{enumerate}
\text Finally, we derived D. \\

\newpage

\section*{Problem 2b}
$KB = \{A \lor B, B \xrightarrow{} C, ( A \lor C) \xrightarrow{} D\}$ \\
\begin{enumerate}[label=(\roman*)]
    \item\text First, let's convert this $KB$ into CNF forms.
        \begin{align*}
            {B \xrightarrow{} C} \quad &\Rightarrow \quad {\neg B \lor C} \\ \\
            {(A \lor C) \xrightarrow{} D} \quad &\Rightarrow \quad { \neg (A \lor C) \lor D} \quad \\&\Rightarrow \quad {(\neg A \land \neg C) \lor D} \quad \\&\Rightarrow \quad {(\neg A \lor D) \land (\neg C \lor D)} \quad \\&\Rightarrow \quad {\neg A \lor D, \neg C \lor D}
        \end{align*}
    $KB = \{{A \lor B}, {\neg B \lor C}, {\neg A \lor D}, {\neg C \lor D}\}$ \\

    \item\text Secondly, let's apply Resolution inference rule. \\
        \begin{align*}
            \frac{A \lor B, \neg B \lor C}{A \lor C} \quad &\Rightarrow \quad KB = \{{A \lor B}, {\neg B \lor C}, {\neg A \lor D}, {\neg C \lor D}, {A \lor C} \} \\
            \frac{A \lor C, \neg C \lor D}{A \lor D} \quad &\Rightarrow \quad KB = \{{A \lor B}, {\neg B \lor C}, {\neg A \lor D}, {\neg C \lor D}, {A \lor C}, {A \lor D} \} \\
            \frac{D \lor \neg A, A \lor D}{D \lor D} \quad &\Rightarrow \quad KB = \{{A \lor B}, {\neg B \lor C}, {\neg A \lor D},{\neg C \lor D}, {A \lor C}, {A \lor D}, {D} \} \\ &(\because \quad D \lor D \Rightarrow D)
        \end{align*}
\end{enumerate}
\text Finally, we derived D. \\

\end{document}
